examples/riscv/isqrt/isqrt_symb_execScript.sml
@@ -89,4 +89,42 @@ val _ = Portable.pprint Tag.pp_tag (tag symb_analysis_thm);
 
 Theorem isqrt_symb_analysis_2_thm = symb_analysis_thm
 
+(* ----------- *)
+(* loop branch *)
+(* ----------- *)
+
+val bprog_tm = (snd o dest_eq o concl) bir_isqrt_prog_def;
+val init_addr_tm = (snd o dest_eq o concl) isqrt_init_addr_3_def;
+val end_addr_tm = (snd o dest_eq o concl) isqrt_end_addr_3_def;
+val birs_state_init_lbl_tm =
+ (snd o dest_eq o concl o EVAL) ``bir_block_pc (BL_Address (Imm64 ^init_addr_tm))``;
+val birs_state_end_lbls =
+ [(snd o dest_eq o concl o EVAL) ``bir_block_pc (BL_Address (Imm64 ^end_addr_tm))``,
+  (snd o dest_eq o concl o EVAL) ``bir_block_pc (BL_Address (Imm64 0x10490w))``];
+val bspec_pre_tm = (lhs o snd o strip_forall o concl) bspec_isqrt_pre_3_def;
+val bprog_envtyl_tm = (fst o dest_eq o concl) isqrt_birenvtyl_def;
+
+val bsysprecond_thm =
+(computeLib.RESTR_EVAL_CONV [``birs_eval_exp``] THENC birs_stepLib.birs_eval_exp_CONV)
+``mk_bsysprecond ^bspec_pre_tm ^bprog_envtyl_tm``;
+val birs_pcond_tm = (snd o dest_eq o concl) bsysprecond_thm;
+
+val timer = bir_miscLib.timer_start 0;
+
+val symb_analysis_thm = bir_symb_analysis
+  bprog_tm birs_state_init_lbl_tm birs_state_end_lbls
+  bprog_envtyl_tm birs_pcond_tm;
+
+val _ = bir_miscLib.timer_stop
+ (fn delta_s => print ("\n======\n > bir_symb_analysis took " ^ delta_s ^ "\n"))
+ timer;
+
+val _ = Portable.pprint Tag.pp_tag (tag bsysprecond_thm);
+
+Theorem isqrt_bsysprecond_3_thm = bsysprecond_thm
+
+val _ = Portable.pprint Tag.pp_tag (tag symb_analysis_thm);
+
+Theorem isqrt_symb_analysis_3_thm = symb_analysis_thm
+
 val _ = export_theory ();
